coq/NNRC/Lang/NNRCSize.v
@@ -14,9 +14,9 @@
  * limitations under the License.
  *)
 
-Section size.
+Section NNRCSize.
   Require Import Omega.
-  Require Import BasicRuntime NNRC.
+  Require Import BasicRuntime cNNRC.
 
   Context {fruntime:foreign_runtime}.
 
@@ -39,7 +39,51 @@ Section size.
     induction n; simpl; omega.
   Qed.
 
-End size.
+  Require Import cNNRCShadow.
+  Require Import EquivDec Decidable.
+  Require Import String.
+
+  Lemma nnrc_rename_lazy_size n x1 x2:
+    nnrc_size (nnrc_rename_lazy n x1 x2) = nnrc_size n.
+  Proof.
+    nnrc_cases (induction n) Case;
+    unfold nnrc_rename_lazy in *;
+    simpl;
+    destruct (equiv_dec x1 x2);
+    simpl;
+    try reflexivity;
+    try solve [ rewrite IHn1;
+                rewrite IHn2;
+                rewrite IHn3;
+                reflexivity ];
+    try solve [ rewrite IHn1;
+                rewrite IHn2;
+                reflexivity ];
+    try solve [ rewrite IHn;
+                reflexivity ];
+    try solve [ rewrite IHn1;
+                destruct (equiv_dec v x1);
+                simpl; try reflexivity;
+                rewrite IHn2;
+                reflexivity ].
+    - Case "NNRCVar"%string.
+      destruct (equiv_dec v x1);
+        simpl; reflexivity.
+    - Case "NNRCEither"%string.
+      rewrite IHn1.
+      destruct (equiv_dec v x1);
+        destruct (equiv_dec v0 x1);
+        simpl; try reflexivity.
+      + rewrite IHn3.
+        reflexivity.
+      + rewrite IHn2.
+        reflexivity.
+      + rewrite IHn2.
+        rewrite IHn3.
+        reflexivity.
+  Qed.
+
+End NNRCSize.
 
 (* 
 *** Local Variables: ***
