coq/NNRC/Typing/TcNNRC.v
@@ -1,0 +1,296 @@
+(*
+ * Copyright 2015-2016 IBM Corporation
+ *
+ * Licensed under the Apache License, Version 2.0 (the "License");
+ * you may not use this file except in compliance with the License.
+ * You may obtain a copy of the License at
+ *
+ * http://www.apache.org/licenses/LICENSE-2.0
+ *
+ * Unless required by applicable law or agreed to in writing, software
+ * distributed under the License is distributed on an "AS IS" BASIS,
+ * WITHOUT WARRANTIES OR CONDITIONS OF ANY KIND, either express or implied.
+ * See the License for the specific language governing permissions and
+ * limitations under the License.
+ *)
+
+Section TcNNRC.
+  Require Import String.
+  Require Import List.
+  Require Import Arith.
+  Require Import Program.
+  Require Import EquivDec Morphisms.
+
+  Require Import Utils BasicSystem.
+  Require Import cNNRC.
+
+  (** Typing rules for NNRC *)
+  Section typ.
+
+    Context {m:basic_model}.
+
+    Inductive nnrc_type : tbindings -> nnrc -> rtype -> Prop :=
+    | TNNRCVar {τ} tenv v : lookup equiv_dec tenv v = Some τ -> nnrc_type tenv (NNRCVar v) τ
+    | TNNRCConst {τ} tenv c : data_type (normalize_data brand_relation_brands c) τ -> nnrc_type tenv (NNRCConst c) τ
+    | TNNRCBinop  {τ₁ τ₂ τ} tenv b e1 e2 :
+        binOp_type b τ₁ τ₂ τ ->
+        nnrc_type tenv e1 τ₁ ->
+        nnrc_type tenv e2 τ₂ ->
+        nnrc_type tenv (NNRCBinop b e1 e2) τ
+    | TNNRCUnop {τ₁ τ} tenv u e1 :
+        unaryOp_type u τ₁ τ ->
+        nnrc_type tenv e1 τ₁ ->
+        nnrc_type tenv (NNRCUnop u e1) τ
+    | TNNRCLet {τ₁ τ₂} v tenv e1 e2 :
+        nnrc_type tenv e1 τ₁ ->
+        nnrc_type ((v,τ₁)::tenv) e2 τ₂ ->
+        nnrc_type tenv (NNRCLet v e1 e2) τ₂
+    | TNNRCFor {τ₁ τ₂} v tenv e1 e2 :
+        nnrc_type tenv e1 (Coll τ₁) ->
+        nnrc_type ((v,τ₁)::tenv) e2 τ₂ ->
+        nnrc_type tenv (NNRCFor v e1 e2) (Coll τ₂)
+    | TNNRCIf {τ} tenv e1 e2 e3 :
+        nnrc_type tenv e1 Bool ->
+        nnrc_type tenv e2 τ ->
+        nnrc_type tenv e3 τ ->
+        nnrc_type tenv (NNRCIf e1 e2 e3) τ
+    | TNNRCEither {τ τl τr} tenv ed xl el xr er :
+        nnrc_type tenv ed (Either τl τr) ->
+        nnrc_type ((xl,τl)::tenv) el τ ->
+        nnrc_type ((xr,τr)::tenv) er τ ->
+        nnrc_type tenv (NNRCEither ed xl el xr er) τ.
+
+  End typ.
+  
+  (** Main lemma for the type correctness of NNNRC *)
+
+  Theorem typed_nnrc_yields_typed_data {m:basic_model} {τ} (env:bindings) (tenv:tbindings) (e:nnrc) :
+    bindings_type env tenv ->
+    nnrc_type tenv e τ ->
+    (exists x, (nnrc_core_eval brand_relation_brands env e) = Some x /\ (data_type x τ)).
+  Proof.
+    intros.
+    revert env H.
+    dependent induction H0; simpl; intros.
+    - unfold bindings_type in *.
+      dependent induction H0.
+      simpl in *; congruence.
+      simpl in *.
+      destruct x; simpl in *.
+      elim H0; clear H0; intros.
+      destruct y; simpl in *.
+      rewrite H0 in *; clear H0.
+      revert H.
+      elim (equiv_dec v s0); intros.
+      exists d.
+      inversion H.
+      rewrite H3 in *; clear H3 H a.
+      split; [reflexivity|assumption].
+      specialize (IHForall2 H); clear H.
+      assumption.
+    - exists (normalize_data brand_relation_brands c).
+      split; [reflexivity|assumption].
+    - specialize (IHnnrc_type1 env H0); specialize (IHnnrc_type2 env H0).
+      elim IHnnrc_type1; intros; clear IHnnrc_type1;
+      elim IHnnrc_type2; intros; clear IHnnrc_type2.
+      elim H1; clear H1; intros.
+      elim H2; clear H2; intros.
+      rewrite H1; rewrite H2.
+      simpl; apply (@typed_binop_yields_typed_data _ _ _ _ _ _ _ _ τ₁ τ₂ τ); assumption.
+    - specialize (IHnnrc_type env H1).
+      elim IHnnrc_type; intros; clear IHnnrc_type.
+      elim H2; clear H2; intros.
+      rewrite H2; clear H2.
+      simpl; apply (@typed_unop_yields_typed_data _ _ _ _ _ _ _ _ τ₁ τ); assumption.
+    - destruct (IHnnrc_type1 _ H) as [?[re1 ?]].
+      destruct (IHnnrc_type2 ((v,x)::env)) as [?[re2 ?]].
+      + apply Forall2_cons; intuition.
+      + unfold var in *.
+        rewrite re1, re2.
+        eauto.
+    - specialize (IHnnrc_type1 env H).
+      elim IHnnrc_type1; intros; clear IHnnrc_type1.
+      elim H0; clear H0; intros.
+      rewrite H0; clear H0; simpl.
+      dependent induction H1.
+      rewrite Forall_forall in *.
+      induction dl; simpl in *.
+      + exists (dcoll []).
+        split; [reflexivity|apply dtcoll; apply Forall_nil].
+      + assert (forall x : data, In x dl -> data_type x r)
+          by (intros; apply (H0 x0); right; assumption).
+        specialize (IHdl H1); clear H1.
+        elim IHdl; intros; clear IHdl.
+        elim H1; clear H1; intros.
+        unfold lift in H1.
+        unfold var in *.
+        assert (exists x1, rmap (fun d1 : data => nnrc_core_eval brand_relation_brands ((v, d1) :: env) e2) dl = Some x1 /\ (dcoll x1) = x0).
+        revert H1.
+        elim (rmap (fun d1 : data => nnrc_core_eval brand_relation_brands ((v, d1) :: env) e2) dl); intros.
+        exists a0; split; try inversion H1; reflexivity.
+        congruence.
+        elim H3; clear H3; intros.
+        elim H3; clear H3; intros.
+        rewrite H3.
+        rewrite <- H4 in *; clear H1 H3 H4; simpl.
+        specialize (IHnnrc_type2 ((v,a)::env)).
+        assert (bindings_type ((v, a) :: env) ((v, τ₁) :: tenv)).
+        unfold bindings_type.
+        apply Forall2_cons; try assumption.
+        simpl; split; try reflexivity.
+        assert (r = τ₁) by (apply rtype_fequal; assumption).
+        rewrite H1 in *; clear H1 x.
+        apply (H0 a); left; reflexivity.
+        specialize (IHnnrc_type2 H1); clear H1.
+        elim IHnnrc_type2; clear IHnnrc_type2; intros.
+        elim H1; clear H1; intros.
+        rewrite H1; simpl.
+        exists (dcoll (x2::x1)); split; try reflexivity.
+        apply dtcoll.
+        rewrite Forall_forall; simpl; intros.
+        elim H4; clear H4; intros.
+        rewrite H4 in *; assumption.
+        dependent induction H2.
+        rewrite Forall_forall in *.
+        assert (r0 = τ₂) by (apply rtype_fequal; assumption).
+        rewrite H5 in *; clear H5.
+        apply (H1 x4); assumption.
+    - specialize (IHnnrc_type1 env H); specialize (IHnnrc_type2 env H); specialize (IHnnrc_type3 env H).
+      elim IHnnrc_type1; intros; clear IHnnrc_type1;
+      elim IHnnrc_type2; intros; clear IHnnrc_type2;
+      elim IHnnrc_type3; intros; clear IHnnrc_type3.
+      elim H0; clear H0; intros.
+      elim H1; clear H1; intros.
+      elim H2; clear H2; intros.
+      rewrite H0.
+      simpl.
+      dependent induction H3.
+      destruct b.
+      + rewrite H1.
+        exists x0; split; [reflexivity|assumption].
+      + rewrite H2.
+        exists x1; split; [reflexivity|assumption].
+    - destruct (IHnnrc_type1 _ H) as [dd [evald typd]].
+      apply data_type_Either_inv in typd.
+      rewrite evald.
+      destruct typd as [[ddl[? typd]]|[ddr[? typd]]]; subst.
+      + destruct (IHnnrc_type2 ((xl,ddl)::env));
+           unfold bindings_type in *; auto.
+      + destruct (IHnnrc_type3 ((xr,ddr)::env));
+           unfold bindings_type in *; auto.
+  Qed.
+
+    (* we are only sensitive to the environment up to lookup *)
+  Global Instance nnrc_type_lookup_equiv_prop {m:basic_model} :
+    Proper (lookup_equiv ==> eq ==> eq ==> iff) nnrc_type.
+  Proof.
+    cut (Proper (lookup_equiv ==> eq ==> eq ==> impl) nnrc_type);
+    unfold Proper, respectful, lookup_equiv, iff, impl; intros; subst;
+      [intuition; eauto | ].
+    rename y0 into e.
+    rename y1 into τ.
+    rename x into b1.
+    rename y into b2.
+    revert b1 b2 τ H H2.
+    induction e; simpl; inversion 2; subst; econstructor; eauto 3.
+    - rewrite <- H; trivial.
+    - eapply IHe2; try eassumption; intros.
+      simpl; match_destr.
+    - eapply IHe2; try eassumption; intros.
+      simpl; match_destr.
+    - eapply IHe2; try eassumption; intros.
+      simpl; match_destr.
+    - eapply IHe3; try eassumption; intros.
+      simpl; match_destr.
+  Qed.
+
+End TcNNRC.
+
+Ltac nnrc_inverter := 
+  match goal with
+    | [H:Coll _ = Coll _ |- _] => inversion H; clear H
+    | [H: proj1_sig ?τ₁ = Coll₀ (proj1_sig ?τ₂) |- _] => rewrite (Coll_right_inv τ₁ τ₂) in H; subst
+    | [H:  Coll₀ (proj1_sig ?τ₂) = proj1_sig ?τ₁ |- _] => symmetry in H
+    (* Note: do not generalize too hastily on unaryOp/binOp constructors *)
+    | [H:nnrc_type _ (NNRCVar _) _ |- _ ] => inversion H; clear H
+    | [H:nnrc_type _ (NNRCConst _) _ |- _ ] => inversion H; clear H
+    | [H:nnrc_type _ (NNRCBinop _ _ _ ) _ |- _ ] => inversion H; clear H
+    | [H:nnrc_type _ (NNRCUnop _ _ ) _ |- _ ] => inversion H; clear H
+    | [H:nnrc_type _ (NNRCLet _ _ _ ) _ |- _ ] => inversion H; clear H
+    | [H:nnrc_type _ (NNRCFor _ _ _ ) _ |- _ ] => inversion H; clear H
+    | [H:nnrc_type _ (NNRCIf _ _ _ ) _ |- _ ] => inversion H; clear H
+    | [H:nnrc_type _ (NNRCEither _ _ _ _ _ ) _ |- _ ] => inversion H; clear H
+    | [H: (_,_)  = (_,_) |- _ ] => inversion H; clear H
+    | [H: map (fun x2 : string * {τ₀ : rtype₀ | wf_rtype₀ τ₀ = true} =>
+                 (fst x2, proj1_sig (snd x2))) ?x0 = nil |- _] => apply (map_rtype_nil x0) in H; simpl in H; subst
+    | [H: (map
+             (fun x : string * {τ₀ : rtype₀ | wf_rtype₀ τ₀ = true} =>
+                (fst x, proj1_sig (snd x))) _)
+          = 
+          (map
+             (fun x : string * {τ₀ : rtype₀ | wf_rtype₀ τ₀ = true} =>
+                (fst x, proj1_sig (snd x))) _) |- _ ] =>
+      apply map_rtype_fequal in H; trivial
+    | [H:Rec _ _ _ = Rec _ _ _ |- _ ] => generalize (Rec_inv H); clear H; intro H; try subst
+    | [H: context [(_::nil) = map 
+                                (fun x : string * {τ₀ : rtype₀ | wf_rtype₀ τ₀ = true} =>
+                                   (fst x, proj1_sig (snd x))) _] |- _] => symmetry in H
+                                                                                         
+    | [H: context [map 
+                     (fun x : string * {τ₀ : rtype₀ | wf_rtype₀ τ₀ = true} =>
+                        (fst x, proj1_sig (snd x))) _ = (_::nil) ] |- _] => apply map_eq_cons in H;
+                                                                            destruct H as [? [? [? [??]]]]
+    | [H:nnrc_type _ _ (snd ?x) |- _ ] => destruct x
+    | [H: Coll₀ _ = Coll₀ _ |- _ ] => inversion H; clear H
+    | [H: Rec₀ _ _ = Rec₀ _ _ |- _ ] => inversion H; clear H
+    | [H:unaryOp_type AColl _ _ |- _ ] => inversion H; clear H; subst
+    | [H:unaryOp_type AFlatten _ _ |- _ ] => inversion H; clear H; subst
+    | [H:unaryOp_type (ARec _) _ _ |- _ ] => inversion H; clear H; subst
+    | [H:unaryOp_type (ADot _) _ _ |- _ ] => inversion H; clear H; subst
+    | [H:unaryOp_type (ARecProject _) _ _ |- _ ] => inversion H; clear H; subst
+    | [H:unaryOp_type (ARecRemove _) _ _ |- _ ] => inversion H; clear H; subst
+    | [H:unaryOp_type ALeft _ _ |- _ ] => inversion H; clear H; subst
+    | [H:unaryOp_type ARight _ _ |- _ ] => inversion H; clear H; subst
+    | [H:binOp_type AConcat _ _ _ |- _ ] => inversion H; clear H
+    | [H:binOp_type AAnd _ _ _ |- _ ] => inversion H; clear H
+    | [H:binOp_type AMergeConcat _ _ _ |- _ ] => inversion H; clear H
+    | [H:context [@equiv_dec ?a ?b ?c ?d ?v ?v] |- _]
+      => destruct (@equiv_dec a b c d v v); [ | congruence]
+    | [H:context [string_eqdec ?v ?v] |- _]
+      => destruct (string_eqdec v v); [ | congruence]
+    | [H:context [string_dec ?v ?v] |- _]
+      => destruct (string_dec v v); [ | congruence]
+    | [H:context [string_dec ?v ?v] |- _]
+      => destruct (string_dec v v); [ | congruence]
+    | [|- context [@equiv_dec ?a ?b ?c ?d ?v ?v] ]
+      => destruct (@equiv_dec a b c d v v); [ | congruence]
+    | [|- context [string_eqdec ?v ?v]]
+      => destruct (string_eqdec v v); [ | congruence]
+    | [|- context [string_dec ?v ?v]]
+      => destruct (string_dec v v); [ | congruence]
+    | [|- context [string_dec ?v ?v]]
+      => destruct (string_dec v v); [ | congruence]
+    | [H:equiv ?v ?v |- _] => clear H
+    | [H:?v = ?v |- _] => clear H
+    | [H:Some _ = Some _ |- _ ]
+      => inversion H; clear H
+  end; try rtype_equalizer; try assumption; try subst; simpl in *; try nnrc_inverter.
+
+  Ltac nnrc_input_well_typed :=
+  repeat progress
+         match goal with
+           | [HO:nnrc_type ?Γ ?op ?τout,
+              HE:bindings_type ?env ?Γ
+              |- context [(nnrc_core_eval brand_relation_brands ?env ?op)]] =>
+             let xout := fresh "dout" in
+             let xtype := fresh "τout" in
+             let xeval := fresh "eout" in
+             destruct (typed_nnrc_yields_typed_data env Γ op HE HO)
+               as [xout [xeval xtype]]; rewrite xeval in *; simpl
+         end.
+
+(* 
+*** Local Variables: ***
+*** coq-load-path: (("../../../coq" "Qcert")) ***
+*** End: ***
+*)
